Ugly WIP of eta-equality proof

theories/LCProps.v
@@ -1,5 +1,6 @@
+Set Primitive Projections.
 From Equations Require Import Equations.
-From OGS Require Import Utils Ctx EventD CatD ITreeD EqD LCD.
+From OGS Require Import Utils Ctx EventD CatD ITreeD EqD AngelicD LCD.
 
 (*********************************************)
 (* Notations for equivalence of lassen trees *)
@@ -106,8 +107,239 @@ Qed.
 (**********************************)
 (* various proofs on lassen trees *)
 
+Equations eq_fin1 (x : Fin.fin 1) : x = Fin.F0 :=
+  eq_fin1 (Fin.F0) := eq_refl.
+
+Equations eq_neg {Γ : neg_ctx} {a b : ty} (i : (Γ : ctx) ∋ (a → b)%ty) : neg_var i = @NArr a b :=
+  eq_neg i with neg_var i := { | NArr := eq_refl } .
+
+From Paco Require Import paco.
+
+Definition unfold_iter {I} {E : event I I} {X Y : I -> Type} (body : X ⇒ᵢ itree E (X +ᵢ Y))
+           {i} (x : X i) 
+           : observe (RecD.iter body i x) = observe (ITreeD.bind (body i x) (fun _ y => match y with
+                             | inl x' => Tau (RecD.iter body _ x')
+                             | inr y => Ret y
+                             end)).
+  reflexivity.
+  Qed.
+
+Definition unfold_iterₐ {I} {E : event I I} {X Y i} (body : X -> itreeₐ E i i (X + Y)) (x : X)
+  : observe (iterₐ body x)
+    = observe (body x !>= fun r => match r with
+                             | inl x => tauₐ (iterₐ body x)
+                             | inr y => retₐ y
+              end).
+  Proof. reflexivity. Qed.
+
+(*
+Definition subst_ret_obs {I} {E : event I I} {X Y} (f : X ⇒ᵢ itree E Y) {i} (x : X i)
+        : observe (subst f (Ret x)) = observe (f i x) := eq_refl.
+
+Definition subst_ret {I} {E : event I I} {X Y} (f : X ⇒ᵢ itree E Y) {i} (x : X i)
+        : subst f (Ret x) = f i x := eq_refl.
+
+  lazy delta beta.
+  lazy iota.
+  replace (Ret x) with ({| _observe := RetF x : itreeF E _ _ i |}).
+Definition subst {I} {E : event I I} {X Y} (f : X ⇒ᵢ itree E Y)
+                 : itree E X ⇒ᵢ itree E Y :=
+*)
+
 Theorem lassen_eta {Γ : neg_ctx} {a b} (i : (Γ : ctx) ∋ (a → b)%ty)
   : Var i ≈L Lam (App (Var (pop i)) (Var top)).
-Admitted.
+
+  (* 1. step *)
+  apply paco3.paco3_fold.
+  unfold eqit_; cbn.
+  econstructor.
+  intros [x v]; revert v.
+  rewrite (eq_fin1 x). cbn. clear x. intro v.
+
+  (* 2. step *)
+  left. apply paco3.paco3_fold.
+  cbn. econstructor. left.
+  cbn [ r_shift has_case ]. cbn.
+  pose (j := @r_concat_l' Γ (a_cext v) (a → b) i). fold j.
+  unfold eval_lassen'.
+
+  (* 3. step *)
+  apply paco3.paco3_fold.
+  rewrite 2 unfold_iter.
+  destruct v.
+  + 
+    cbn [ t_of_a fst snd ].
+    unfold eval_enf, bindₐ, sub, MonadItree.
+    cbv [ bind RecD.emb_comp iterₐ ].
+    unfold bindₐ.
+    unfold sub.
+    unfold MonadItree.
+    cbn.
+    rewrite 2 unfold_iterₐ.
+    cbn [ eval_enf ].
+
+  (* expand lots of stuff (too much) *)
+  lazy beta delta [RecD.iter ].
+  cbn [ fst snd
+         MonadItree Basics.compose pin
+         observe _observe
+         bind subst sub
+         ret AngelicD.retₐ tau AngelicD.tauₐ fiber_into
+         RecD.iter RecD.emb_comp RecD.translate_fwd
+         eval_enf
+         AngelicD.bindₐ AngelicD.iterₐ AngelicD.ret₀
+         e_focus
+         ].
+
+  (** Left branch **)
+  (* compute through focus_aux *)
+  rewrite focus_aux.focus_aux_equation_4,
+          focus_aux.focus_aux_equation_1,
+          focus_aux.focus_aux_equation_11,
+          focus_aux.focus_aux_equation_1,
+          focus_aux.focus_aux_equation_12.
+
+  (* compute through eval_aux *)
+  rewrite eval_aux_equation_2,
+          lassen_enf_equation_2,
+          (eq_neg j),  (* unstuck trivial proof *)
+          lassen_enf_clause_2_equation_1.
 
 
+  (** Right branch **)
+  rewrite focus_aux.focus_aux_equation_4.
+  rewrite focus_aux.focus_aux_equation_2.
+  rewrite focus_aux.focus_aux_equation_11.
+  rewrite focus_aux.focus_aux_equation_1.
+  rewrite focus_aux.focus_aux_equation_12.
+  rewrite eval_aux_equation_3.
+  cbn.
+  fold (@focus_aux.focus_aux Γ).
+  econstructor; auto.
+  econstructor.
+  
+  Locate "/ₛ".
+  unfold t_subst1.
+  unfold t_subst1_clause_1_f.
+  simpl t_subst.
+  Search eval_aux.
+                         eval_aux
+                           (ERed EHole (VLam (App (Var (pop j)) (Var top)))
+                              (RApp (VVar top)))
+  rewrite eval_aux_equation_1.
+  rewrite lassen_enf_equation_2.
+
+  
+                           (focus_aux.focus_aux EHole
+                              (inl
+                                 (App (Lam (App (Var (pop j)) (Var top))) (Var top))))
+  change (neg_var j) with (@NArr (a → b0) b).
+  simpl lassen_enf.
+  cbn.
+  Search lassen_enf_clause_2
+  Search "focus_aux".
+  (focus_aux.focus_aux EHole (inl (App (Var j) (Var top))))
+                                 Subterm.FixWf Fix Fix_F wellfounded
+                                 Telescopes.wf_tele_measure Subterm.lt_wf Wf.measure_wf ].
+  unfold eval_enf.
+
+
+
+
+  RecD.emb_comp RecD.translate_fwd 
+                         AngelicD.bindₐ AngelicD.iterₐ AngelicD.ret₀
+                         AngelicD.tauₐ tau AngelicD.retₐ 
+                         ret tau vis
+                         eval_enf
+                         fiber_into
+                         MonadItree Basics.compose pin
+                         e_focus focus_aux.focus_aux ].
+  lazy iota beta delta [ observe _observe
+                         bind subst sub
+                         RecD.iter RecD.emb_comp RecD.translate_fwd 
+                         AngelicD.bindₐ AngelicD.iterₐ AngelicD.ret₀
+                         AngelicD.tauₐ tau AngelicD.retₐ 
+                         ret tau vis
+                         eval_enf
+                         fiber_into
+                         MonadItree Basics.compose pin
+                         e_focus focus_aux.focus_aux ].
+  cbn.
+  unfold lassen_enf_clause_2.
+  lazy iota beta.
+  lazy iota beta delta [ r_concat_l' r_concat_l eq_rect_r ].
+  unfold r_concat_l'.
+  Search "lassen_enf_clause_2".
+  lazy delta [ eval_enf ].
+  Locate "=<<".
+  Check sub.
+  
+  cbn.
+  lazy iota beta delta [ eval_enf ].
+  lazy iota beta delta [ observe ].
+.  lazy iota beta delta -[ observe RecD.iter subst fiber_into RecD.emb_comp ].
+  lazy iota beta zeta delta [ r_shift has_case apply_noConfusion noConfusion_retr noConfusion_inv noConfusion NoConfusion ].
+  lazy iota beta zeta delta [ observe RecD.iter ].
+  lazy iota beta delta [ observe RecD.iter ].
+  unfold observe.
+  cbn.
+  destruct v.
+  unfold t_of_a.
+  unfold eval_enf.
+  cbn.
+  unfold r_shift.
+  lazy iota beta delta [ has_case ].
+  cbn.
+  cbn.
+  
+  
+  Locate (_ \/)
+  apply paco3.upaco3_mon_bot.
+  Search paco3.upaco3.
+  unfold lassen_val, subst.
+  cbn.
+  repeat lazy cofix.
+  lazy beta match cofix.
+  simpl.
+  lazy.
+  lazy beta iota.
+  
+  Print go.
+  Print
+  replace (Ret (inl (EA EHole (apply_obs (VVar i) v)))) with ({| _observe := RetF (inl (EA EHole (apply_obs (VVar i) v))) |} : lassen (eval_arg' +ᵢ ∅ᵢ) _).
+  compute.
+  vm_compute.
+  unfold lassen_val.
+  unfold subst.
+  unfold observe.
+
+
+  unfold subst.
+  cbn.
+  cbn
+  cbn in v.
+  destruct v.
+  cbn.
+  destruct x.
+  case x.
+  unfold enf_k_rsp in v.
+
+  destruct x.
+  cbn in v.
+  destruct (u_rsp enf_e (LVal (@AArr Γ a b) : u_qry enf_e (_ , _))).
+  Check subst
+  cbn in v.
+  edestruct v as [n x].
+  cbn.
+  destruct n.
+  cbn in x.
+  cbn in k.
+  destruct x.
+  destruct x.
+  unfold id.
+  Search paco3.upaco3.
+  cbn in v.
+
+  From Coq Require Import Morphisms.
+  Check eqitF.
+  Check (Proper _ )
